testdata/cue/comprehensions/comprehension_embed_self_narrow_body.cue
@@ -1,0 +1,3 @@
+#H: {#t: string | *"def"}
+#R: Self={#H, out: [for x in [1] {v: Self.#t}]}
+v: #R & {#t: "y"}
